Progress on [lemma_eval_ins_equiv_states]

vale/code/lib/transformers/Vale.Transformers.InstructionReorder.fst
@@ -274,6 +274,71 @@ let lemma_untainted_eval_ins_equiv_states (i : ins) (s1 s2 : machine_state) :
   | Dealloc _ ->
     assert_spinoff (equiv_states_ext s1_final s2_final)
 
+let rec lemma_taint_match_args_equiv_states
+  (args:list instr_operand)
+  (oprs:instr_operands_t_args args)
+  (memTaint:memTaint_t)
+  (stackTaint:memTaint_t)
+  (s1 s2:machine_state) :
+  Lemma
+    (requires (equiv_states s1 s2))
+    (ensures (
+        (taint_match_args args oprs memTaint stackTaint s1) ==
+        (taint_match_args args oprs memTaint stackTaint s2))) =
+  match args with
+  | [] -> ()
+  | i :: args ->
+    match i with
+    | IOpEx i ->
+      let oprs : instr_operand_t i & instr_operands_t_args args = coerce oprs in
+      lemma_taint_match_args_equiv_states args (snd oprs) memTaint stackTaint s1 s2
+    | IOpIm i ->
+      lemma_taint_match_args_equiv_states args (coerce oprs) memTaint stackTaint s1 s2
+
+let rec lemma_taint_match_inouts_equiv_states
+  (inouts:list instr_out)
+  (args:list instr_operand)
+  (oprs:instr_operands_t inouts args)
+  (memTaint:memTaint_t)
+  (stackTaint:memTaint_t)
+  (s1 s2:machine_state) :
+  Lemma
+    (requires (equiv_states s1 s2))
+    (ensures (
+        (taint_match_inouts inouts args oprs memTaint stackTaint s1) ==
+        (taint_match_inouts inouts args oprs memTaint stackTaint s2))) =
+  match inouts with
+  | [] -> lemma_taint_match_args_equiv_states args oprs memTaint stackTaint s1 s2
+  | (Out, i) :: inouts ->
+    let oprs =
+      match i with
+      | IOpEx i -> snd #(instr_operand_t i) (coerce oprs)
+      | IOpIm i -> coerce oprs
+    in
+    lemma_taint_match_inouts_equiv_states inouts args oprs memTaint stackTaint s1 s2
+  | (InOut, i)::inouts ->
+    let (v, oprs) =
+      match i with
+      | IOpEx i ->
+        let oprs = coerce oprs in
+        (taint_match_operand_explicit i (fst oprs) memTaint stackTaint s1, snd oprs)
+      | IOpIm i -> (taint_match_operand_implicit i memTaint stackTaint s1, coerce oprs)
+    in
+    lemma_taint_match_inouts_equiv_states inouts args oprs memTaint stackTaint s1 s2
+
+let lemma_taint_match_ins_equiv_states (i : ins) (s1 s2 : machine_state) :
+  Lemma
+    (requires (equiv_states s1 s2))
+    (ensures (
+        (taint_match_ins i s1.ms_memTaint s1.ms_stackTaint s1) ==
+        (taint_match_ins i s2.ms_memTaint s2.ms_stackTaint s2))) =
+  match i with
+  | Instr (InstrTypeRecord #outs #args _) oprs _ ->
+    assert (s1.ms_memTaint == s2.ms_memTaint);
+    assert (s1.ms_stackTaint == s2.ms_stackTaint);
+    lemma_taint_match_inouts_equiv_states outs args oprs s1.ms_memTaint s1.ms_stackTaint s1 s2
+  | Push _ _ | Pop _ _ | Alloc _ | Dealloc _ -> ()
+
 let lemma_eval_ins_equiv_states (i : ins) (s1 s2 : machine_state) :
   Lemma
     (requires (equiv_states s1 s2))
@@ -283,7 +348,8 @@ let lemma_eval_ins_equiv_states (i : ins) (s1 s2 : machine_state) :
           (machine_eval_ins i s2))) =
   let s10 = run (check (taint_match_ins i s1.ms_memTaint s1.ms_stackTaint)) s1 in
   let s20 = run (check (taint_match_ins i s2.ms_memTaint s2.ms_stackTaint)) s2 in
-  assume (equiv_states s10 s20);
+  lemma_taint_match_ins_equiv_states i s1 s2;
+  assert (equiv_states s10 s20);
   let memTaint1, stackTaint1 = update_taint_ins i s1.ms_memTaint s1.ms_stackTaint s10 in
   let memTaint2, stackTaint2 = update_taint_ins i s2.ms_memTaint s2.ms_stackTaint s20 in
   assume (memTaint1 == memTaint2);
